Rename whnf_red_shape_spec and some small fixes
whnf_red_shape_spec -> whnf_red
whnf_red_shape -> whnf_red_inv

pcuic/theories/PCUICNormal.v
@@ -889,66 +889,149 @@ Qed.
 
 Hint Resolve All2_same All2_firstn All2_skipn OnOne2_All2 red_mkApps All2_app : pcuic.
 
-Inductive whnf_red_shape_spec Σ Γ : term -> term -> Prop :=
-| wr_shape_tRel i :
+(* For terms in whnf we have a very useful inversion lemma for reductions.
+   This next relation is a subrelation of red that classifies how whnf terms reduce. *)
+Inductive whnf_red Σ Γ : term -> term -> Prop :=
+| whnf_red_tRel i :
     option_map decl_body (nth_error Γ i) = Some None ->
-    whnf_red_shape_spec Σ Γ (tRel i) (tRel i)
-| wr_shape_tVar id : whnf_red_shape_spec Σ Γ (tVar id) (tVar id)
-| wr_shape_tEvar n l l' :
+    whnf_red Σ Γ (tRel i) (tRel i)
+| whnf_red_tVar id : whnf_red Σ Γ (tVar id) (tVar id)
+| whnf_red_tEvar n l l' :
     All2 (red Σ Γ) l l' ->
-    whnf_red_shape_spec Σ Γ (tEvar n l) (tEvar n l')
-| wr_shape_tConst kn u decl :
+    whnf_red Σ Γ (tEvar n l) (tEvar n l')
+| whnf_red_tConst kn u decl :
     lookup_env Σ kn = Some (ConstantDecl decl) ->
     cst_body decl = None ->
-    whnf_red_shape_spec Σ Γ (tConst kn u) (tConst kn u)
-| wr_shape_tApp hd hd' arg arg' :
+    whnf_red Σ Γ (tConst kn u) (tConst kn u)
+| whnf_red_tApp hd hd' arg arg' :
     red Σ Γ hd hd' ->
-    whnf_red_shape_spec Σ Γ hd hd' ->
+    whnf_red Σ Γ hd hd' ->
     red Σ Γ arg arg' ->
-    whnf_red_shape_spec Σ Γ (tApp hd arg) (tApp hd' arg')
-| wr_shape_tFix mfix mfix' idx :
+    whnf_red Σ Γ (tApp hd arg) (tApp hd' arg')
+| whnf_red_tFix mfix mfix' idx :
     All2 (fun d d' => dname d = dname d' ×
                       rarg d = rarg d' ×
                       red Σ Γ (dtype d) (dtype d') ×
                       red Σ (Γ,,, fix_context mfix) (dbody d) (dbody d'))
          mfix mfix' ->
-    whnf_red_shape_spec Σ Γ (tFix mfix idx) (tFix mfix' idx)
-| wr_shape_tCase p motive motive' discr discr' brs brs' :
+    whnf_red Σ Γ (tFix mfix idx) (tFix mfix' idx)
+| whnf_red_tCase p motive motive' discr discr' brs brs' :
     red Σ Γ motive motive' ->
     red Σ Γ discr discr' ->
     All2 (fun br br' => br.1 = br'.1 × red Σ Γ br.2 br'.2) brs brs' ->
-    whnf_red_shape_spec Σ Γ (tCase p motive discr brs) (tCase p motive' discr' brs')
-| wr_shape_tProj p c c' :
+    whnf_red Σ Γ (tCase p motive discr brs) (tCase p motive' discr' brs')
+| whnf_red_tProj p c c' :
     red Σ Γ c c' ->
-    whnf_red_shape_spec Σ Γ (tProj p c) (tProj p c')
-| wr_shape_tSort s : whnf_red_shape_spec Σ Γ (tSort s) (tSort s)
-| wr_shape_tProd na A A' B B' :
+    whnf_red Σ Γ (tProj p c) (tProj p c')
+| whnf_red_tSort s : whnf_red Σ Γ (tSort s) (tSort s)
+| whnf_red_tProd na A A' B B' :
     red Σ Γ A A' ->
     red Σ (Γ,, vass na A) B B' ->
-    whnf_red_shape_spec Σ Γ (tProd na A B) (tProd na A' B')
-| wr_shape_tLambda na A A' B B' :
+    whnf_red Σ Γ (tProd na A B) (tProd na A' B')
+| whnf_red_tLambda na A A' B B' :
     red Σ Γ A A' ->
     red Σ (Γ,, vass na A) B B' ->
-    whnf_red_shape_spec Σ Γ (tLambda na A B) (tLambda na A' B')
-| wr_shape_tConstruct i n u :
-    whnf_red_shape_spec Σ Γ (tConstruct i n u) (tConstruct i n u)
-| wr_shape_tInd i u :
-    whnf_red_shape_spec Σ Γ (tInd i u) (tInd i u)
-| wr_shape_tCoFix mfix mfix' idx :
+    whnf_red Σ Γ (tLambda na A B) (tLambda na A' B')
+| whnf_red_tConstruct i n u :
+    whnf_red Σ Γ (tConstruct i n u) (tConstruct i n u)
+| whnf_red_tInd i u :
+    whnf_red Σ Γ (tInd i u) (tInd i u)
+| whnf_red_tCoFix mfix mfix' idx :
     All2 (fun d d' => dname d = dname d' ×
                       rarg d = rarg d' ×
                       red Σ Γ (dtype d) (dtype d') ×
                       red Σ (Γ,,, fix_context mfix) (dbody d) (dbody d'))
          mfix mfix' ->
-    whnf_red_shape_spec Σ Γ (tCoFix mfix idx) (tCoFix mfix' idx).
+    whnf_red Σ Γ (tCoFix mfix idx) (tCoFix mfix' idx).
 
-Derive Signature for whnf_red_shape_spec.
+Derive Signature for whnf_red.
 
-Instance whnf_red_shape_spec_trans Σ Γ : RelationClasses.Transitive (whnf_red_shape_spec Σ Γ).
+Lemma whnf_red_red Σ Γ t t' :
+  whnf_red Σ Γ t t' ->
+  ∥red Σ Γ t t'∥.
+Proof.
+  intros wh.
+  depelim wh; constructor; eauto with pcuic.
+  - apply red_evar; auto.
+  - apply red_app; auto.
+  - apply red_fix_congr.
+    eapply All2_impl; eauto.
+    cbn.
+    intros ? ? (->&->&r1&r2).
+    eauto.
+  - apply red_case; auto.
+    eapply All2_impl; eauto.
+    cbn.
+    intros ? ? (->&?).
+    eauto.
+  - apply red_proj_c; auto.
+  - apply red_prod; auto.
+  - apply red_abs; auto.
+    eapply context_change_decl_types_red; eauto.
+    constructor; [|constructor].
+    apply context_relation_refl.
+    reflexivity.
+  - apply red_cofix_congr.
+    eapply All2_impl; eauto.
+    cbn.
+    intros ? ? (->&->&r1&r2).
+    eauto.
+Qed.
+
+Lemma whnf_red_mkApps Σ Γ hd hd' args args' :
+  whnf_red Σ Γ hd hd' ->
+  red Σ Γ hd hd' ->
+  All2 (red Σ Γ) args args' ->
+  whnf_red Σ Γ (mkApps hd args) (mkApps hd' args').
+Proof.
+  intros shape r ra.
+  induction ra using All2_ind_rev; auto.
+  rewrite <- !mkApps_nested.
+  cbn.
+  constructor; auto.
+  apply red_mkApps; auto.
+Qed.
+
+Lemma whnf_red_refl_whne Σ Γ t :
+  whne RedFlags.default Σ Γ t ->
+  whnf_red Σ Γ t t.
+Proof.
+  intros wh.
+  induction wh; cbn in *; try discriminate; eauto using whnf_red with pcuic.
+  apply whnf_red_mkApps; auto.
+  2: apply All2_same; auto.
+  constructor.
+  apply All2_same; auto.
+Qed.
+
+Lemma whnf_red_refl Σ Γ t :
+  whnf RedFlags.default Σ Γ t ->
+  whnf_red Σ Γ t t.
+Proof.
+  intros wh.
+  induction wh; cbn in *; try discriminate; eauto using whnf_red with pcuic.
+  - eapply whnf_red_refl_whne; eauto.
+  - apply whnf_red_mkApps; auto.
+    2: apply All2_same; auto.
+    constructor.
+  - apply whnf_red_mkApps; auto.
+    2: apply All2_same; auto.
+    constructor.
+  - apply whnf_red_mkApps; auto.
+    2: apply All2_same; auto.
+    constructor.
+    apply All2_same; auto.
+  - apply whnf_red_mkApps; auto.
+    2: apply All2_same; auto.
+    constructor.
+    apply All2_same; auto.
+Qed.
+
+Instance whnf_red_trans Σ Γ : RelationClasses.Transitive (whnf_red Σ Γ).
 Proof.
   intros x y z xy yz.
   revert z yz.
-  induction xy; intros z yz; depelim yz; eauto using whnf_red_shape_spec.
+  induction xy; intros z yz; depelim yz; eauto using whnf_red.
   - constructor.
     eapply All2_trans; eauto.
     typeclasses eauto.
@@ -997,49 +1080,23 @@ Proof.
     now apply All2_length in X.
 Qed.
 
-Lemma whnf_red_shape_spec_mkApps Σ Γ hd hd' args args' :
-  whnf_red_shape_spec Σ Γ hd hd' ->
-  red Σ Γ hd hd' ->
-  All2 (red Σ Γ) args args' ->
-  whnf_red_shape_spec Σ Γ (mkApps hd args) (mkApps hd' args').
-Proof.
-  intros shape r ra.
-  induction ra using All2_ind_rev; auto.
-  rewrite <- !mkApps_nested.
-  cbn.
-  constructor; auto.
-  apply red_mkApps; auto.
-Qed.
-
-Lemma whnf_red_shape_spec_refl_whne Σ Γ t :
-  whne RedFlags.default Σ Γ t ->
-  whnf_red_shape_spec Σ Γ t t.
-Proof.
-  intros wh.
-  induction wh; cbn in *; try discriminate; eauto using whnf_red_shape_spec with pcuic.
-  apply whnf_red_shape_spec_mkApps; auto.
-  2: apply All2_same; auto.
-  constructor.
-  apply All2_same; auto.
-Qed.
-
-Lemma whne_red1_shape Σ Γ t t' :
+Lemma whne_red1_inv Σ Γ t t' :
   whne RedFlags.default Σ Γ t ->
   red1 Σ Γ t t' ->
-  whnf_red_shape_spec Σ Γ t t'.
+  whnf_red Σ Γ t t'.
 Proof.
   intros wh r.
   apply (whne_red1_ind
            RedFlags.default Σ Γ
-           (whnf_red_shape_spec Σ Γ)); intros; cbn in *; try easy; eauto using whnf_red_shape_spec.
+           (whnf_red Σ Γ)); intros; cbn in *; try easy; eauto using whnf_red.
   - constructor.
     eapply OnOne2_All2; eauto.
   - constructor; auto.
-    now apply whnf_red_shape_spec_refl_whne.
-  - apply whnf_red_shape_spec_mkApps; eauto.
+    now apply whnf_red_refl_whne.
+  - apply whnf_red_mkApps; eauto.
     1: constructor; apply All2_same; auto.
     eapply OnOne2_All2; eauto.
-  - apply whnf_red_shape_spec_mkApps; eauto.
+  - apply whnf_red_mkApps; eauto.
     + constructor.
       eapply OnOne2_All2; eauto.
       cbn.
@@ -1047,7 +1104,7 @@ Proof.
       auto.
     + now apply red1_red, fix_red_ty.
     + apply All2_same; auto.
-  - apply whnf_red_shape_spec_mkApps; eauto.
+  - apply whnf_red_mkApps; eauto.
     + constructor.
       eapply OnOne2_All2; eauto.
       cbn.
@@ -1064,55 +1121,32 @@ Proof.
     intros ? ? (?&?); auto.
 Qed.
 
-Lemma whnf_red_shape_spec_refl Σ Γ t :
-  whnf RedFlags.default Σ Γ t ->
-  whnf_red_shape_spec Σ Γ t t.
-Proof.
-  intros wh.
-  induction wh; cbn in *; try discriminate; eauto using whnf_red_shape_spec with pcuic.
-  - eapply whnf_red_shape_spec_refl_whne; eauto.
-  - apply whnf_red_shape_spec_mkApps; auto.
-    2: apply All2_same; auto.
-    constructor.
-  - apply whnf_red_shape_spec_mkApps; auto.
-    2: apply All2_same; auto.
-    constructor.
-  - apply whnf_red_shape_spec_mkApps; auto.
-    2: apply All2_same; auto.
-    constructor.
-    apply All2_same; auto.
-  - apply whnf_red_shape_spec_mkApps; auto.
-    2: apply All2_same; auto.
-    constructor.
-    apply All2_same; auto.
-Qed.
-
-Lemma whnf_red1_shape Σ Γ t t' :
+Lemma whnf_red1_inv Σ Γ t t' :
   whnf RedFlags.default Σ Γ t ->
   red1 Σ Γ t t' ->
-  whnf_red_shape_spec Σ Γ t t'.
+  whnf_red Σ Γ t t'.
 Proof.
   intros wh r.
   destruct wh.
-  - eapply whne_red1_shape; eauto.
+  - eapply whne_red1_inv; eauto.
   - depelim r; solve_discr.
-  - depelim r; solve_discr; constructor; eauto using whnf_red_shape_spec.
-  - depelim r; solve_discr; constructor; eauto using whnf_red_shape_spec.
+  - depelim r; solve_discr; constructor; eauto using whnf_red.
+  - depelim r; solve_discr; constructor; eauto using whnf_red.
   - apply red1_mkApps_tConstruct_inv in r as (?&->&?).
-    apply whnf_red_shape_spec_mkApps; eauto using whnf_red_shape_spec.
+    apply whnf_red_mkApps; eauto using whnf_red.
     eapply OnOne2_All2; eauto.
   - apply red1_mkApps_tInd_inv in r as (?&->&?).
-    apply whnf_red_shape_spec_mkApps; eauto using whnf_red_shape_spec.
+    apply whnf_red_mkApps; eauto using whnf_red.
     eapply OnOne2_All2; eauto.
   - apply red1_mkApps_tFix_inv in r.
     2: { destruct unfold_fix as [(?&?)|]; [|easy].
          now unfold is_constructor; rewrite H. }
     destruct r as [[(?&->&?)|(?&->&?)]|(?&->&?)].
-    + apply whnf_red_shape_spec_mkApps; auto.
+    + apply whnf_red_mkApps; auto.
       2: eapply OnOne2_All2; eauto.
       constructor.
       apply All2_same; auto.
-    + apply whnf_red_shape_spec_mkApps.
+    + apply whnf_red_mkApps.
       3: apply All2_same; auto.
       2: apply red1_red, fix_red_ty; auto.
       constructor.
@@ -1120,7 +1154,7 @@ Proof.
       cbn.
       intros ? ? (?&[= -> -> ->]).
       auto.
-    + apply whnf_red_shape_spec_mkApps.
+    + apply whnf_red_mkApps.
       3: apply All2_same; auto.
       2: apply red1_red, fix_red_body; auto.
       constructor.
@@ -1130,11 +1164,11 @@ Proof.
       auto.
   - apply red1_mkApps_tCoFix_inv in r.
     destruct r as [[(?&->&?)|(?&->&?)]|(?&->&?)].
-    + apply whnf_red_shape_spec_mkApps; auto.
+    + apply whnf_red_mkApps; auto.
       2: eapply OnOne2_All2; eauto.
       constructor.
       apply All2_same; auto.
-    + apply whnf_red_shape_spec_mkApps.
+    + apply whnf_red_mkApps.
       3: apply All2_same; auto.
       2: apply red1_red, cofix_red_ty; auto.
       constructor.
@@ -1142,7 +1176,7 @@ Proof.
       cbn.
       intros ? ? (?&[= -> -> ->]).
       auto.
-    + apply whnf_red_shape_spec_mkApps.
+    + apply whnf_red_mkApps.
       3: apply All2_same; auto.
       2: apply red1_red, cofix_red_body; auto.
       constructor.
@@ -1152,15 +1186,15 @@ Proof.
       auto.
 Qed.
 
-Lemma whnf_red_shape Σ Γ t t' :
+Lemma whnf_red_inv Σ Γ t t' :
   whnf RedFlags.default Σ Γ t ->
   red Σ Γ t t' ->
-  whnf_red_shape_spec Σ Γ t t'.
+  whnf_red Σ Γ t t'.
 Proof.
   intros wh r.
   induction r using red_rect_n1.
-  - apply whnf_red_shape_spec_refl; auto.
-  - eapply whnf_red1_shape in X.
+  - apply whnf_red_refl; auto.
+  - eapply whnf_red1_inv in X.
     + etransitivity; eauto.
     + eapply whnf_pres; eauto.
 Qed.
@@ -1171,7 +1205,7 @@ Lemma whnf_red_isApp Σ Γ t t' :
   isApp t' = isApp t.
 Proof.
   intros wh r.
-  eapply whnf_red_shape in r; eauto.
+  eapply whnf_red_inv in r; eauto.
   now depelim r.
 Qed.
 
@@ -1182,7 +1216,7 @@ Lemma whnf_red_mkApps_l Σ Γ hd args t :
     t = mkApps hd' args' × red Σ Γ hd hd' × All2 (red Σ Γ) args args'∥.
 Proof.
   intros wh r.
-  eapply whnf_red_shape in wh; eauto.
+  eapply whnf_red_inv in wh; eauto.
   induction args in hd, t, r, wh |- * using List.rev_ind.
   - cbn in *.
     constructor; eexists _, []; split; [reflexivity|].
@@ -1204,7 +1238,7 @@ Lemma whnf_red_mkApps_r Σ Γ t hd' args' :
     t = mkApps hd args × red Σ Γ hd hd' × All2 (red Σ Γ) args args'∥.
 Proof.
   intros wh r.
-  eapply whnf_red_shape in wh; eauto.
+  eapply whnf_red_inv in wh; eauto.
   induction args' in hd', t, r, wh |- * using List.rev_ind.
   - cbn in *.
     constructor; eexists _, []; split; [reflexivity|].
@@ -1219,7 +1253,7 @@ Proof.
     eauto with pcuic.
 Qed.
 
-Lemma whnf_red_mkApps Σ Γ hd args hd' args' :
+Lemma whnf_red_mkApps_inv Σ Γ hd args hd' args' :
   whnf RedFlags.default Σ Γ (mkApps hd args) ->
   red Σ Γ (mkApps hd args) (mkApps hd' args') ->
   isApp hd = false ->
@@ -1267,14 +1301,6 @@ Proof.
     now rewrite nth_error_nil in H0.
 Qed.
 
-Lemma whne_eq_term {cf:checker_flags} f Σ φ Γ t t' :
-  whne f Σ Γ t ->
-  eq_term Σ φ t t' ->
-  whne f Σ Γ t'.
-Proof.
-  apply whne_eq_term_upto_univ_napp.
-Qed.
-
 Lemma whnf_eq_term_upto_univ_napp f Σ Γ t Re Rle napp t' :
   whnf f Σ Γ t ->
   eq_term_upto_univ_napp Σ Re Rle napp t t' ->
@@ -1318,308 +1344,3 @@ Lemma whnf_eq_term {cf:checker_flags} f Σ φ Γ t t' :
 Proof.
   apply whnf_eq_term_upto_univ_napp.
 Qed.
-
-(* 
-
-  Definition head_arg_is_constructor mfix idx args :=
-    match unfold_fix mfix idx with Some (narg, body) => is_constructor narg args | None => false end.
-  
-
-  Inductive normal (Γ : context) : term -> Prop :=
-  | nf_ne t : neutral Γ t -> normal Γ t
-  | nf_lam na A B : normal Γ A -> normal (Γ ,, vass na A) B ->
-                    normal Γ (tLambda na A B)
-  | nf_cstrapp i n u v : All (normal Γ) v -> normal Γ (mkApps (tConstruct i n u) v)
-  | nf_indapp i u v : All (normal Γ) v -> normal Γ (mkApps (tInd i u) v)
-  | nf_fix mfix idx args : All (compose (normal (Γ ,,, PCUICLiftSubst.fix_context mfix)) dbody) mfix ->
-                           All (normal Γ) args ->
-                           head_arg_is_constructor mfix idx args = false ->
-                           All (compose (normal Γ) dtype) mfix ->
-                      normal Γ (mkApps (tFix mfix idx) args)
-  | nf_cofix mfix idx : All (compose (normal (Γ ,,, PCUICLiftSubst.fix_context mfix)) dbody) mfix ->
-                      All (compose (normal Γ) dtype) mfix ->
-                        normal Γ (tCoFix mfix idx)
-
-  with neutral (Γ : context) : term -> Prop :=
-  | ne_rel i :
-      (forall b, option_map decl_body (nth_error Γ i) <> Some (Some b)) ->
-      neutral Γ (tRel i)
-  | ne_var v : neutral Γ (tVar v)
-  | ne_evar n l : neutral Γ (tEvar n l)
-  | ne_const c u :
-      (forall decl b, lookup_env Σ c = Some (ConstantDecl decl) -> decl.(cst_body) = Some b -> False) ->
-      neutral Γ (tConst c u)
-  | ne_sort s : neutral Γ (tSort s)
-  | ne_prod na A B : normal Γ A -> normal (Γ ,, vass na A) B ->
-                     neutral Γ (tProd na A B)
-  | ne_app f v : neutral Γ f -> normal Γ v -> neutral Γ (tApp f v)
-  | ne_case i p c brs : neutral Γ c -> normal Γ p -> All (compose (normal Γ) snd) brs ->
-                        neutral Γ (tCase i p c brs)
-  | ne_proj p c : neutral Γ c -> neutral Γ (tProj p c).
-
-Definition normal_neutral_dec Σ Γ t : ({normal Σ Γ t} + {~ (normal Σ  Γ t)}) * ({neutral Σ Γ t} + {~ (neutral Σ Γ t)}).
-Proof.
-  induction t using term_forall_mkApps_ind in Γ |- *; split; eauto.
-  all: try now (right; intros H; depelim H).
-  - destruct (option_map decl_body (nth_error Γ n)) as [ [ | ] | ] eqn:E.
-    + right. intros H. depelim H. depelim H. congruence. help. help. help.
-    + eauto.
-    + right. intros H. depelim H. depelim H. congruence. help. help. help.
-  - destruct (option_map decl_body (nth_error Γ n)) as [ [ | ] | ] eqn:E.
-    + right. intros H. depelim H. congruence.
-    + eauto.
-    + right. intros H. depelim H. congruence.
-  - todo "evar".
-  - todo "evar".
-  - destruct (IHt1 Γ) as [[] _];
-      [destruct (IHt2 (Γ,, vass n t1)) as [[] _]|]; eauto.
-    + right. intros H. depelim H. depelim H. eauto. help. help. help.
-    + right. intros H. depelim H. depelim H. eauto. help. help. help.
-  - destruct (IHt1 Γ) as [[] _];
-      [destruct (IHt2 (Γ,, vass n t1)) as [[] _]|]; eauto.
-    + right. intros H. depelim H. eauto. 
-    + right. intros H. depelim H. eauto.
-  - destruct (IHt1 Γ) as [[] _];
-      [destruct (IHt2 (Γ,, vass n t1)) as [[] _]|]; eauto.
-    + right. intros H. depelim H. depelim H. eauto. help. help. help.
-    + right. intros H. depelim H. depelim H. eauto. help. help. help.
-  - right. intros H. depelim H. depelim H. help. help. help.
-  - destruct (IHt Γ) as [[] _].
-    + destruct dec_All with (P := (normal Σ Γ)) (L := v).
-      -- eapply All_impl. eassumption. intros ? ?. apply X0.
-      -- destruct t. all:eauto using normal_mkApps, All_Forall.
-         all: try now (left; depelim n; help; eauto).
-         ++ destruct v as [ | ? v].
-            ** eauto.
-            ** right. todo "admit". (*  intros ?. depelim X. depelim X. all:help. clear IHt. *)
-               (* eapply neutral_mk_Apps_inv in H0. as []; eauto. *)
-               (* depelim H1. *)
-         ++ destruct (head_arg_is_constructor mfix idx v) eqn:E.
-            ** right. intros ?. todo "admit". (* depelim H1. depelim H1. all:help. clear IHv. *)
-               (* eapply neutral_mk_Apps_inv in H1 as []; eauto. depelim H1. *)
-            ** left. todo "admit". (* depelim n. all:help. depelim H1. *)
-               (* eapply (f_equal decompose_app) in x; *)
-               (*   rewrite !decompose_app_mkApps in x; cbn in *; try firstorder congruence.  inv x. *)
-               (* eauto. *)
-         ++ todo "cofix".
-      -- right. intros ?. eapply f. eapply Forall_All.
-         now eapply normal_mk_Apps_inv.
-    + right. intros ?. eapply n. now eapply normal_mk_Apps_inv.
-  - destruct v using rev_ind.
-    + cbn. eapply IHt.
-    + rewrite <- mkApps_nested. cbn.
-      eapply All_app in X as []. eapply IHv in a. inv a0. clear X0.
-      rename X into IHt2.
-      revert a.
-      generalize (mkApps t v) as t1. intros t1 IHt1.
-      destruct (IHt1) as [];
-      [destruct (IHt2 Γ) as [[] _]|]; eauto.
-      * right. intros HH. depelim HH. eauto.
-      * right. intros HH. depelim HH. eauto.
-  - destruct (lookup_env Σ s) as [[] | ] eqn:E.
-    + destruct (cst_body c) eqn:E2.
-      * right. intros H. depelim H. depelim H. congruence. help. help. help.
-      * eauto. 
-    +   right. intros H. depelim H. depelim H. congruence. help. help. help.
-    +   right. intros H. depelim H. depelim H. congruence. help. help. help.
-  - destruct (lookup_env Σ s) as [[] | ] eqn:E.
-    + destruct (cst_body c) eqn:E2.
-      * right. intros H. depelim H. congruence.
-      * eauto. 
-    +   right. intros H. depelim H. congruence.
-    +   right. intros H. depelim H. congruence.
-  - left. eapply nf_indapp with (v := []). econstructor.
-  - left. eapply nf_cstrapp with (v := []). econstructor.
-  - destruct (IHt2 Γ) as [_ []].
-    + destruct (IHt1 Γ) as [[] _].
-      * destruct dec_All with(L := l) (P := (normal Σ Γ ∘ @snd nat term)).
-        -- eapply All_impl. eassumption. intros ? ?. eapply X0.
-        -- eauto.
-        -- right. intros ?. depelim H. depelim H. all:help. eauto.
-      * right. intros ?. depelim H. depelim H. all:help. eauto.
-    + right. intros ?. depelim H. depelim H. all:help. eauto.
-  -  destruct (IHt2 Γ) as [_ []].
-    + destruct (IHt1 Γ) as [[] _].
-      * destruct dec_All with(L := l) (P := (normal Σ Γ ∘ @snd nat term)).
-        -- eapply All_impl. eassumption. intros ? ?. eapply X0.
-        -- eauto.
-        -- right. intros ?. depelim H. all:help. eauto.
-      * right. intros ?. depelim H. all:help. eauto.
-    + right. intros ?. depelim H. all:help. eauto.
-  - destruct (IHt Γ) as [_ []].
-    + eauto.
-    + right. intros H. depelim H. depelim H. eauto. help. help. help.
-  - destruct (IHt Γ) as [_ []].
-    + eauto.
-    + right. intros H. depelim H. eauto.
-  - hnf in X.
-
-    destruct dec_All with (P := (normal Σ Γ ∘ dtype)) (L := m).
-    eapply All_impl. eassumption. cbn. intros. eapply X0.
-
-    destruct dec_All with (P := normal Σ  (Γ ,,, PCUICLiftSubst.fix_context m) ∘ dbody) (L := m).
-    eapply All_impl. exact X. cbn. intros. eapply X0.
-
-    + left. eapply nf_fix with (args := []). eauto. eauto. unfold head_arg_is_constructor.
-      destruct unfold_fix; eauto. destruct p.
-      unfold is_constructor. destruct n0; eauto. eauto.
-    + right. intros H. depelim H. depelim H. help. help. eapply f.
-      eapply (f_equal decompose_app) in x;
-        rewrite !decompose_app_mkApps in x; cbn in *; try firstorder congruence.  inv x.
-      eauto.
-    + right. intros H. depelim H. depelim H. help. help. 
-      eapply (f_equal decompose_app) in x;
-        rewrite !decompose_app_mkApps in x; cbn in *; try firstorder congruence.  inv x.
-      eauto.      
-  - hnf in X.
-
-    destruct dec_All with (P := (normal Σ Γ ∘ dtype)) (L := m).
-    eapply All_impl. eassumption. cbn. intros. eapply X0.
-
-    destruct dec_All with (P := normal Σ (Γ ,,, PCUICLiftSubst.fix_context m) ∘ dbody) (L := m).
-    eapply All_impl. exact X. cbn. intros. eapply X0.
-
-    + left. eapply nf_cofix. eauto. eauto.
-    + right. intros H. depelim H. depelim H. help. help. help. eauto.
-    + right. intros H. depelim H. depelim H. help. help. help. eauto.
-Defined.
-
-Definition normal_dec Σ Γ t := fst (normal_neutral_dec Σ Γ t).
-Definition neutral_dec Σ Γ t := snd (normal_neutral_dec Σ Γ t).
- *)
-
-
-(* 
-
-
-Lemma OnOn2_contra A  (P : A -> A -> Type) l1 l2 : (forall x y, P x y -> False) -> OnOne2 P l1 l2 -> False.
-Proof.
-  intros. induction X; eauto.
-Qed.
-
-Lemma normal_nf Σ Γ t t' : normal Σ Γ t \/ neutral Σ Γ t -> red1 Σ Γ t t' -> False.
-Proof.
-  intros. induction X using red1_ind_all; destruct H.
-  all: repeat match goal with
-         | [ H : normal _ _ (?f ?a) |- _ ] => depelim H
-         | [ H : neutral _ _ (?f ?a)|- _ ] => depelim H
-         end.
-  all: try congruence.
-  all: help.
-  all: try tauto.
-  all: try now (clear - H; depind H; help; eauto).
-  - eapply (f_equal decompose_app) in x;
-      rewrite !decompose_app_mkApps in x; cbn in *; try firstorder congruence.
-    inv x. unfold head_arg_is_constructor in H.
-    rewrite H0 in H. congruence.
-  - eapply OnOne2_All_mix_left in X; try eassumption.
-    eapply OnOn2_contra; try eassumption.
-    firstorder.
-  - eapply OnOne2_All_mix_left in X; try eassumption.
-    eapply OnOn2_contra; try eassumption.
-    firstorder.
-  - eapply IHX. left.
-    eapply nf_cstrapp. now eapply All_app in X as [X _].
-  - eapply IHX. left.
-    eapply nf_indapp. now eapply All_app in X as [X _].
-  - clear IHargs.
-    eapply IHX. left.
-    eapply nf_fix.
-    + eauto.
-    + eapply All_app in X0. eapply X0.
-    + unfold head_arg_is_constructor in *.
-      destruct unfold_fix; eauto. destruct p.
-      unfold is_constructor in *.
-      destruct (nth_error args n) eqn:E; eauto.
-      erewrite nth_error_app_left in H; eauto.
-    + eauto.
-  - eapply IHX. left.
-    eapply All_app in X as [_ X]. now inv X.
-  - eapply IHX. left.
-    eapply All_app in X as [_ X]. now inv X.
-  - eapply IHX. left.
-    eapply All_app in X0 as [_ X0]. now inv X0.
-  - eapply OnOne2_All_mix_left in X; try eassumption.
-    eapply OnOn2_contra; try eassumption.
-    firstorder.
-  - eapply OnOne2_All_mix_left in X; try eassumption.
-    eapply OnOn2_contra; try eassumption.
-    firstorder.
-  - eapply (f_equal decompose_app) in x;
-      rewrite !decompose_app_mkApps in x; cbn in *; try firstorder congruence. inv x.
-    eapply OnOne2_All_mix_left in X; try eassumption.
-    eapply OnOn2_contra; try eassumption.
-(*     firstorder. *)
-(*   - eapply (f_equal decompose_app) in x; *)
-(*       rewrite !decompose_app_mkApps in x; cbn in *; try firstorder congruence. inv x. *)
-(*     eapply OnOne2_All_mix_left in X. 2:exact H. *)
-(*     eapply OnOn2_contra; try eassumption. *)
-(*     firstorder. *)
-(*   - eapply OnOne2_All_mix_left in X. 2:exact H0. *)
-(*     eapply OnOn2_contra; try eassumption. *)
-(*     firstorder. *)
-(*   - eapply OnOne2_All_mix_left in X. 2:exact H. *)
-(*     eapply OnOn2_contra; try eassumption. *)
-(*     firstorder. *)
-(* Qed. *)
-Admitted.
-
-Hint Constructors normal neutral : core.
-
-Lemma normal_mk_Apps_inv:
-  forall (Σ : global_env) (Γ : context) (t : term) (v : list term), ~ isApp t -> normal Σ Γ (mkApps t v) -> normal Σ Γ t /\ Forall (normal Σ Γ) v.
-Proof.
-(*   intros Σ Γ t v H H1. *)
-(*   induction v using rev_ind. *)
-(*   - split. eapply H1. econstructor.  *)
-(*   - rewrite <- mkApps_nested in H1. cbn in H1. depelim H1. depelim H0. *)
-(*     + split. *)
-(*       * firstorder. *)
-(*       * eapply app_Forall. firstorder. firstorder. *)
-(*     + change (tApp (mkApps t v) x0) with (mkApps (mkApps t v) [x0]) in *. *)
-(*       rewrite mkApps_nested in x. *)
-(*       eapply (f_equal decompose_app) in x. *)
-(*       rewrite !decompose_app_mkApps in x; cbn in *; try congruence. firstorder. inv x. *)
-(*       split. eapply nf_cstrapp with (v := []). econstructor. *)
-(*       now eapply All_Forall.  *)
-(*     + change (tApp (mkApps t v) x0) with (mkApps (mkApps t v) [x0]) in *. *)
-(*       rewrite mkApps_nested in x. *)
-(*       eapply (f_equal decompose_app) in x. *)
-(*       rewrite !decompose_app_mkApps in x; cbn in *; try congruence. firstorder. inv x. *)
-(*       split. eapply nf_indapp with (v := []). econstructor. *)
-(*       now eapply All_Forall. *)
-(*     + change (tApp (mkApps t v) x0) with (mkApps (mkApps t v) [x0]) in *. *)
-(*       rewrite mkApps_nested in x. *)
-(*       eapply (f_equal decompose_app) in x. *)
-(*       rewrite !decompose_app_mkApps in x; cbn in *; try congruence. firstorder. inv x. *)
-(*       split. eapply nf_fix with (args := []). *)
-(*       * eauto. *)
-(*       * econstructor. *)
-(*       * unfold head_arg_is_constructor in *. *)
-(*         destruct unfold_fix; eauto. destruct p. *)
-(*         unfold is_constructor in *. destruct n; reflexivity. *)
-(*       * eauto. *)
-(*       * now eapply All_Forall. *)
-(* Qed. *)
-Admitted.
-
-Lemma neutral_mk_Apps_inv:
-  forall (Σ : global_env) (Γ : context) (t : term) (v : list term), ~ isApp t -> neutral Σ Γ (mkApps t v) -> neutral Σ Γ t /\ Forall (normal Σ Γ) v.
-Proof.
-  intros Σ Γ t v H H1.
-  induction v using rev_ind.
-  - split. eapply H1. econstructor. 
-  - rewrite <- mkApps_nested in H1. cbn in H1. depelim H1. 
-    split.
-    + firstorder.
-    + eapply app_Forall. firstorder. firstorder.
-Qed.
-
-Lemma normal_mkApps Σ Γ t v :
-  neutral Σ Γ t -> Forall (normal Σ Γ) v -> normal Σ Γ (mkApps t v).
-Proof.
-  intros. induction H0 in t, H |- *; cbn in *.
-  - eauto.
-  - eapply IHForall. eauto.
-Qed.  
- *)
